alphaeq.v
@@ -739,6 +739,116 @@ Proof using.
     eauto.
 Qed.
 
+
+Let uniqVarLb :BTerm -> list NVar * list BTerm -> list NVar * list BTerm 
+:= (fun (b : BTerm) (r : list NVar * list BTerm) =>
+              let (rlv, rb) := r in
+              (bound_vars_bterm (uniq_change_bvars_alphabt rlv b)++ rlv,
+              uniq_change_bvars_alphabt rlv b :: rb)).
+
+Lemma uniqVarLbFst : forall lbt lv, 
+let (rlv, rbt) := fold_right uniqVarLb (lv,[]) lbt in
+rlv = flat_map bound_vars_bterm rbt ++ lv.
+Proof.
+  induction lbt; intros; simpl; auto; autorewrite with list.
+  specialize (IHlbt lv).
+  destruct (fold_right uniqVarLb (lv, []) lbt).
+  unfold uniqVarLb. simpl.  subst l.
+  rewrite app_assoc.
+  refl.
+Qed.
+
+Lemma uniq_change_bvars_alpha_spec_aux:
+  (forall nt  lv, 
+  let nt' := uniq_change_bvars_alpha lv nt in
+  NoDup (bound_vars nt') # disjoint lv (bound_vars nt') #alpha_eq nt nt')
+  * (forall bt  lv,
+  let (blv, bnt) := uniq_change_bvars_alphabt lv bt in
+  let bt' := bterm blv bnt in
+  NoDup (bound_vars_bterm bt') # disjoint lv (bound_vars_bterm bt') #alpha_eq_bterm bt bt').
+Proof using.
+  intros. apply NTerm_BTerm_ind;
+    [intro v; cpx| |].
+- intros ? ? Hind.
+  simpl.
+  induction lbt as [| b lbt]; simpl; [intros; dands; cpx;
+  constructor; cpx; fail|].
+  simpl. intros lv. simpl in *.
+  pose proof (uniqVarLbFst lbt lv) as Hbt.
+  unfold uniqVarLb in Hbt.
+  specialize (IHlbt (fun b inb => Hind b (or_intror inb)) lv).
+  destruct(fold_right
+                       (fun (b : BTerm) (r : list NVar * list BTerm) =>
+                        let (rlv, rb) := r in
+                        (bound_vars_bterm (uniq_change_bvars_alphabt rlv b) ++ rlv,
+                        uniq_change_bvars_alphabt rlv b :: rb)) 
+                       (lv, []) lbt) as [rlv rnt].
+  specialize (Hind b ltac:(cpx) rlv).
+  simpl in *.
+  destruct (uniq_change_bvars_alphabt rlv b ) as [blv bnt].
+  subst rlv. repnd.
+  dands.
+  + simpl in *. repnd.
+    apply NoDupApp; auto.
+    repeat disjoint_reasoning.
+
+  + simpl.
+    repeat disjoint_reasoning.
+
+  + constructor; try (rw map_length; auto);[].
+      introv Hlt. rw @selectbt_map; auto.
+      pose proof (selectbt_in2 n lbt Hlt) as XX; exrepnd.
+      destruct bt as [blv bnt]. rewrite XX0.
+      apply Hind. auto.
+
+- intros blv bnt Hnt. split.
+   +  introv Hin Hinc. rename t into vv.
+      allsimpl. subst.
+      simpl in *.
+       addFreshVarsSpec2 vn pp.
+      exrepnd. allsimpl.
+      duplicate Hin.
+      repnd.
+      apply Hnt0 in Hin0.
+      setoid_rewrite boundvars_ssubst_aux_vars in Hinc; sp.
+      apply disjoint_sym  in pp1.
+      apply disjoint_app_l in pp1. repnd. apply pp2 in Hin.
+      apply in_app_iff in Hinc.
+      simpl in *.  
+      dorn Hinc; sp.
+  
+
+  +  allsimpl. subst.
+     simpl. addFreshVarsSpec2 vn pp.
+      destruct (fresh_vars (length blv) (lv ++ vn ++ (all_vars bnt) 
+        ++ all_vars
+     (change_bvars_alpha lv bnt))) as [lvn pal].
+    exrepnd. allsimpl.
+    disjoint_reasoningv.
+     apply al_bterm with (lv:=lvn); sp.
+    unfold all_vars. rw @boundvars_ssubst_aux_vars;sp;
+    try(disjoint_reasoningv).
+    introv Hin Hinc.
+    applydup pal5 in Hin.
+    apply free_vars_ssubst_aux in Hinc;
+    [ |apply disjoint_bv_vars; sp].
+    dorn Hinc; exrepnd; sp. apply in_var_ren in Hinc0. exrepnd.
+    subst.
+    allsimpl.
+    dorn Hinc1; sp.
+    subst.
+    apply pal3 in Hin. sp.
+    rewrite <- ssubst_ssubst_aux; 
+    spcls; disjoint_reasoningv. rewrite ssubst_nest_vars_same; sp;
+    try congruence; try disjoint_reasoningv.
+    apply alpha_eq_if3 with (lv:=nil).
+    change_to_ssubst_aux8.
+    apply alpha3_ssubst_aux_allvars_congr2;sp.
+    Focus 2. disjoint_reasoningv.
+    apply alpha_eq3_if.
+    eauto.
+Qed.
+
 Definition change_bvars_alpha_spec: forall (nt : NTerm) (lv : list NVar),
        disjoint lv (bound_vars (change_bvars_alpha lv nt)) # alpha_eq nt (change_bvars_alpha lv nt)
  := fun nt lv => (fst (change_bvars_alpha_spec_aux lv)) nt.
